thys/First_Order_Terms/Term_More.thy
@@ -2526,6 +2526,10 @@ lemma set_vars_term_list [simp]:
   "set (vars_term_list t) = vars_term t"
   by (induct t) simp_all
 
+lemma vars_term_code[code]:
+  \<open>vars_term t = set (vars_term_list t)\<close>
+  by simp
+
 lemma mset_vars_term_list[simp]: "mset (vars_term_list r) = vars_term_ms r" 
 proof (induct r)
   case (Fun f rs)
